Split general logic, demo logic, and example into different theories

Forward_Hoare.thy
@@ -5,13 +5,97 @@ theory Forward_Hoare
 begin
 
 ML \<open>
+signature HOARE_LOGIC_ARGS =
+sig
+type program
+type range
+val binding: binding
+val read_program: Proof.context -> string -> program
+val read_range: Proof.context -> string -> range
+val valid_range: program -> range -> bool
+(* Contract: valid range *)
+val extract_range: program -> range -> term
+val hoare_thm : Proof.context -> term -> term -> term -> term (* pre prog post *)
+end
+
+datatype ex_program = Ex_Program of exn
+datatype ex_range = Ex_Range of exn
+
+type logic = {
+  binding: binding,
+  serial: serial,
+  read_program: Proof.context -> string -> ex_program,
+  read_range: Proof.context -> string -> ex_range,
+  valid_range: ex_program -> ex_range -> bool,
+  extract_range: ex_program -> ex_range -> term,
+  hoare_thm: Proof.context -> term -> term -> term -> term
+}
+
+structure Logic_Data = Theory_Data(
+  type T = logic Symtab.table
+  val empty = Symtab.empty
+  val merge = Symtab.merge (fn (x,y) => #serial x = #serial y)
+  val extend = I
+)
+
+signature HOARE_LOGIC =
+sig
+type program
+type range
+val logic: logic
+val ex_program : program -> ex_program
+val program_ex : ex_program -> program
+val ex_range : range -> ex_range
+val range_ex : ex_range -> range
+end
+
+functor Hoare_Logic(Logic: HOARE_LOGIC_ARGS): HOARE_LOGIC =
+struct
+
+type program = Logic.program
+type range = Logic.range
+exception Program of program
+exception Range of range
+
+fun err str = error (Binding.name_of Logic.binding ^ "." ^ str)
+
+fun read_program ctxt str = Ex_Program (Program (Logic.read_program ctxt str))
+fun ex_program prog = Ex_Program (Program prog)
+fun program_ex (Ex_Program (Program prog)) = prog
+  | program_ex (Ex_Program e) = err ("program_ex: " ^ \<^make_string> e)
+
+fun read_range ctxt str = Ex_Range (Range (Logic.read_range ctxt str))
+fun ex_range prog = Ex_Range (Range prog)
+fun range_ex (Ex_Range (Range prog)) = prog
+  | range_ex (Ex_Range e) = err ("range_ex: " ^ \<^make_string> e)
+
+fun valid_range prog range = Logic.valid_range (program_ex prog) (range_ex range)
+fun extract_range prog range = Logic.extract_range (program_ex prog) (range_ex range)
+
+val logic : logic = {
+  serial = serial(),
+  binding = Logic.binding,
+  read_program = read_program,
+  read_range = read_range,
+  extract_range = extract_range,
+  valid_range = valid_range,
+  hoare_thm = Logic.hoare_thm
+}
+
+val _ = Context.>> (Context.map_theory (Logic_Data.map (Symtab.update_new (Binding.name_of Logic.binding, logic))))
+end
+
+fun get_logic thy name = Symtab.lookup (Logic_Data.get thy) name
+fun get_logic' ctxt = get_logic (Proof_Context.theory_of ctxt)
+\<close>
+
+ML \<open>
 fun def' binding t lthy =
-  let val ((const,_),lthy) = Local_Theory.define ((binding,NoSyn),((Binding.suffix_name "_def" binding,[]),Thm.term_of t)) lthy
+  let val ((const,_),lthy) = Local_Theory.define ((binding,NoSyn),((Binding.suffix_name "_def" binding,[]),t)) lthy
   in (const,lthy) end
 fun def binding t lthy = def' binding t lthy |> snd
 \<close>
 
-section \<open>Programs\<close>
 type_synonym var = String.literal
 type_synonym mem = \<open>var \<Rightarrow> int\<close>
 datatype instruction = Add var var | Set var int | Guess var
@@ -19,48 +103,15 @@ type_synonym program = "instruction list"
 
 ML \<open>
 type var = string
-datatype instruction = Add of var*var | Set of var*int | Guess of var
-type program = instruction list
-fun instruction_to_term (Set (x, i)) = \<^const>\<open>Set\<close> $ HOLogic.mk_literal x $ HOLogic.mk_number HOLogic.intT i
-  | instruction_to_term (Guess x) = \<^const>\<open>Guess\<close> $ HOLogic.mk_literal x
-  | instruction_to_term (Add (x,y)) = \<^const>\<open>Add\<close> $ HOLogic.mk_literal x $ HOLogic.mk_literal y
-fun program_to_term p = map instruction_to_term p |> HOLogic.mk_list \<^typ>\<open>instruction\<close>
-fun program_to_cterm ctxt p = program_to_term p |> Thm.cterm_of ctxt
+type program = { binding: binding, code: ex_program, logic: string }
+(* fun program_to_cterm ctxt p = program_to_term p |> Thm.cterm_of ctxt *)
 \<close>
 
-section \<open>Invariants\<close>
-
-type_synonym invariant = "mem \<Rightarrow> bool"
-
-fun postcondition_trivial :: "instruction \<Rightarrow> invariant \<Rightarrow> invariant" where
-  "postcondition_trivial (Set x i) I = (\<lambda>m. m x = i \<and> (\<exists>j. I (m(x:=j))))"
-| "postcondition_trivial (Guess x) I = (\<lambda>m. \<exists>j. I (m(x:=j)))"
-| "postcondition_trivial (Add x y) I = (\<lambda>m. I (m(x:=m x - m y)))"
-
-fun postcondition_pick :: "instruction \<Rightarrow> int \<Rightarrow> invariant \<Rightarrow> invariant" where
-  "postcondition_pick (Guess x) i I = (\<lambda>m. m x = i \<and> (\<exists>j. I (m(x:=j))))"
-| "postcondition_pick _ _ _ = undefined"
-
-section \<open>Ranges\<close>
-
-ML \<open>
-type range = int * int
-fun valid_range (program:program) ((start,endd):range) =
-  start <= endd andalso start >= 0 andalso endd <= length program
-(* Contract: valid_range = true *)
-fun extract_range (program:program) ((start,endd):range) : program =
-  program |> drop start |> take (endd-start)
-(* Contract: valid_range = true *)
-fun merge_ranges (_:program) ((s1,e1):range) ((s2,e2):range) : range option =
-  if e1=s2 then SOME (s1,e2) else NONE
-\<close>
-
-section \<open>Joint stuff\<close>
 
 ML \<open>
 type invariant = {
   binding: binding,
-  cterm: cterm,
+  term: term,
   const: term
 }
 \<close>
@@ -69,8 +120,8 @@ type invariant = {
 ML \<open>
 type hoare = {
   binding: binding,
-  range: range,
-  program_fragment: program,
+  range: ex_range,
+  program: string,
   program_fragment_const: term,
   precondition: string,
   postcondition: string,
@@ -81,8 +132,12 @@ type hoare = {
 ML \<open>
 structure Hoare_Data = Proof_Data (
   type T = { invariants: invariant Symtab.table,
-             hoares: hoare Symtab.table }
-  fun init _ = { invariants=Symtab.empty, hoares=Symtab.empty }
+             hoares: hoare Symtab.table,
+             programs: program Symtab.table,
+             current_program: string option
+  }
+  fun init _ = { invariants=Symtab.empty, hoares=Symtab.empty,
+    programs=Symtab.empty, current_program=NONE }
 )
 \<close>
 
@@ -94,44 +149,57 @@ fun mk_the t = let val oT = fastype_of t in case oT of
 \<close>
 
 ML \<open>
-fun map_invariants f = Hoare_Data.map (fn {invariants,hoares} => {invariants=f invariants, hoares=hoares})
-fun map_hoares f = Hoare_Data.map (fn {invariants,hoares} => {invariants=invariants, hoares=f hoares})
+fun map_invariants f = Hoare_Data.map (fn {invariants,hoares,programs,current_program} => 
+  {invariants=f invariants, hoares=hoares, programs=programs, current_program=current_program})
+fun map_hoares f = Hoare_Data.map (fn {invariants,hoares,programs,current_program} => 
+  {invariants=invariants, hoares=f hoares, programs=programs, current_program=current_program})
+fun map_programs f = Hoare_Data.map (fn {invariants,hoares,programs,current_program} => 
+  {invariants=invariants, hoares=hoares, programs=f programs, current_program=current_program})
+fun set_current_program name = Hoare_Data.map (fn {invariants,hoares,programs,current_program=_} => 
+  {invariants=invariants, hoares=hoares, programs=programs, current_program=SOME name})
 fun add_invariant0 i = map_invariants (Symtab.update_new (Binding.name_of (#binding i), i))
 fun add_hoare0 i = map_hoares (Symtab.update_new (Binding.name_of (#binding i), i))
+fun add_program0 p ctxt = let
+  val name = Binding.name_of (#binding p)
+  val ctxt = map_programs (Symtab.update_new (name, p)) ctxt
+  val ctxt = set_current_program name ctxt
+  in ctxt end
 fun get_invariant ctxt name = Symtab.lookup (Hoare_Data.get ctxt |> #invariants) name
 fun get_hoare ctxt name = Symtab.lookup (Hoare_Data.get ctxt |> #hoares) name
+fun get_program ctxt name = Symtab.lookup (Hoare_Data.get ctxt |> #programs) name
+fun get_current_program ctxt = Hoare_Data.get ctxt |> #current_program
 \<close>
 
 ML \<open>
-fun add_invariant binding invariant ctxt : invariant * Proof.context = let
+fun add_invariant binding (invariant:term) ctxt : invariant * Proof.context = let
   fun bind suffix = Binding.suffix_name suffix binding
-  val _ = tracing ("Adding invariant "^ Pretty.string_of (Binding.pretty binding) ^ ": " ^ Syntax.string_of_term ctxt (Thm.term_of invariant))
+  val _ = tracing ("Adding invariant "^ Pretty.string_of (Binding.pretty binding) ^ ": " ^ Syntax.string_of_term ctxt invariant)
   val (invariant_const,ctxt) = def' (bind "_inv") invariant ctxt
-  val info : invariant = {binding=binding, const=invariant_const, cterm=invariant}
+  val info : invariant = {binding=binding, const=invariant_const, term=invariant}
   val ctxt = add_invariant0 info ctxt
   in (info,ctxt) end
 \<close>
 
 ML \<open>
-fun add_hoare1 binding program range (precondition:invariant) (postcondition:invariant) ctxt = let
+fun add_hoare1 binding (program:program) range (precondition:invariant) (postcondition:invariant) (ctxt:Proof.context) = let
   fun bind suffix = Binding.suffix_name suffix binding
-  val program_fragment = extract_range program range
-  val program_fragment_ct = program_to_cterm ctxt program_fragment
-  val _ = tracing ("Program fragment: " ^ Syntax.string_of_term ctxt (Thm.term_of program_fragment_ct))
+  val logic = get_logic (Proof_Context.theory_of ctxt) (#logic program) |> the
+  val program_fragment = (#extract_range logic) (#code program) range
+  (* val program_fragment_ct = program_to_term program_fragment *)
+  val _ = tracing ("Program fragment: " ^ Syntax.string_of_term ctxt program_fragment)
   val (program_fragment_const,ctxt) = 
-      def' (bind "_prog") program_fragment_ct ctxt
+      def' (bind "_prog") program_fragment ctxt
   val info : hoare = {binding=binding, range=range,
     precondition=Binding.name_of (#binding precondition),
     postcondition=Binding.name_of (#binding postcondition),
-    program_fragment=program_fragment, program_fragment_const=program_fragment_const,
+    program_fragment_const=program_fragment_const,
+    program=program |> #binding |> Binding.name_of,
     valid= @{thm TrueI}
   }
   (* val ctxt = add_hoare0 info ctxt *)
   in (info,ctxt) end
 \<close>
 
-
-definition "pc_imp pc1 pc2 \<longleftrightarrow> (\<forall>m. pc1 m \<longrightarrow> pc2 m)"
 
 section \<open>Experiments\<close>
 
@@ -140,10 +208,6 @@ structure Do_Prf = Proof_Data(
   type T = Proof.state -> Proof.state
   fun init _ = fn _ => error "don't call this"
 )
-\<close>
-
-ML \<open>
-val test_prog = [Set ("x", 5), Guess "y", Add ("x", "y")] 
 \<close>
 
 ML \<open>
@@ -170,227 +234,30 @@ ML \<open>
 Proof.have true NONE after_qed [] [] [((binding,[]),[(prop,[])])] true state |> \<^print> |> snd
 \<close>
 
-
-lemma False
-proof -
-  do_prf \<open>fn state => let 
-fun after_qed (ctxt,thms) state = state
-val state = prove \<^binding>\<open>xxxx\<close> after_qed \<^prop>\<open>1=1\<close> state
-in state end
-\<close>
-    by auto
-  thm xxxx
-  oops
-
-lemma pc_impI[intro]: "(\<And>m. pc1 m \<Longrightarrow> pc2 m) \<Longrightarrow> pc_imp pc1 pc2"
-  unfolding pc_imp_def by auto
-
-lemma pc_impD[dest]: "pc_imp pc1 pc2 \<Longrightarrow> pc1 m \<Longrightarrow> pc2 m"
-  unfolding pc_imp_def by auto
-
-
-definition "independent_of (B::invariant) (x::var) = (\<forall>m1 m2. (\<forall>y\<noteq>x. m1 y = m2 y) \<longrightarrow> B m1 = B m2)"
-lemma independent_ofI: 
-  assumes "\<And>m1 m2. (\<And>y. y\<noteq>x \<Longrightarrow> m1 y = m2 y) \<Longrightarrow> B m1 = B m2"
-  shows "independent_of B x"
-  unfolding independent_of_def using assms by metis
-
-lemma newvalue_Set:
-  assumes "invariant \<equiv> postcondition_trivial (Set x i) A"
-  shows "pc_imp invariant (\<lambda>m. m x = i)"
-  unfolding assms
-  by (rule pc_impI; simp)
-
-lemma newvalue_Guess: 
-  assumes "invariant \<equiv> postcondition_pick (Guess x) i A"
-  shows "pc_imp invariant (\<lambda>m. m x = i)"
-  unfolding assms
-  by (rule pc_impI; simp)
-
-lemmas newvalue = newvalue_Set newvalue_Guess
-
-lemma unchanged_Guess_trivial: 
-  assumes "invariant \<equiv> postcondition_trivial (Guess x) A"
-  assumes indep: "independent_of B x"
-  assumes imp: "\<And>m. A m \<Longrightarrow> B m"
-  shows "pc_imp invariant B"
-  unfolding assms(1)
-  apply (rule pc_impI; simp)
-  using indep imp unfolding independent_of_def apply auto
-  by (metis fun_upd_def)+
-
-lemma unchanged_Guess_pick: 
-  assumes "invariant \<equiv> postcondition_pick (Guess x) i A"
-  assumes indep: "independent_of B x"
-  assumes imp: "\<And>m. A m \<Longrightarrow> B m"
-  shows "pc_imp invariant B"
-  unfolding assms(1)
-  apply (rule pc_impI; simp)
-  using indep imp unfolding independent_of_def apply auto
-  by (metis fun_upd_def)+
-
-lemma unchanged_Add: 
-  assumes "invariant \<equiv> postcondition_trivial (Add x y) A"
-  assumes indep: "independent_of B x"
-  assumes xy: "x \<noteq> y"
-  assumes imp: "\<And>m. A m \<Longrightarrow> B m"
-  shows "pc_imp invariant B"
-  unfolding assms
-  apply (rule pc_impI)
-  using indep imp xy unfolding independent_of_def apply auto
-  by (metis fun_upd_def)
-
-lemma unchanged_Set: 
-  assumes "invariant \<equiv> postcondition_trivial (Set x i) A"
-  assumes indep: "independent_of B x"
-  assumes imp: "\<And>m. A m \<Longrightarrow> B m"
-  shows "pc_imp invariant B"
-  unfolding assms(1)
-  apply (rule pc_impI)
-  using indep imp unfolding independent_of_def apply auto
-  by (metis fun_upd_def)
-
-lemmas unchanged = unchanged_Guess_pick unchanged_Guess_trivial unchanged_Add unchanged_Set
-
-lemma wp_Add: 
-  assumes "invariant \<equiv> postcondition_trivial (Add x y) A"
-  assumes distinct: "x \<noteq> y"
-  assumes imp: "\<And>m. A m \<Longrightarrow> B (m(x:=m x + m y))"
-  shows "pc_imp invariant B"
-  unfolding assms(1)
-  apply (rule pc_impI)
-  using distinct apply simp apply (drule imp)
-  by auto
-
-lemma wp_Set:
-  assumes "invariant \<equiv> postcondition_trivial (Set x i) A"
-  assumes imp: "\<And>m. A m \<Longrightarrow> B (m(x:=i))"
-  shows "pc_imp invariant B"
-  unfolding assms(1)
-  apply (rule pc_impI)
-  apply simp
-  using imp
-  apply auto
-  apply (drule imp)
-  by auto
-
-lemmas wp = wp_Add wp_Set
-
-fun semantics1 :: "instruction \<Rightarrow> mem \<Rightarrow> mem set" where
-  "semantics1 (Set x i) m = {m(x:=i)}"
-| "semantics1 (Add x y) m = {m(x:=m x + m y)}"
-| "semantics1 (Guess x) m = {m(x:=i)| i. True}"
-
-fun semantics :: "program \<Rightarrow> mem \<Rightarrow> mem set" where
-  "semantics [] m = {m}"
-| "semantics (c#p) m = (\<Union>m'\<in>semantics1 c m. semantics p m')"
-
-definition hoare :: "invariant \<Rightarrow> program \<Rightarrow> invariant \<Rightarrow> bool" where
-  "hoare A p B \<longleftrightarrow> (\<forall>m. A m \<longrightarrow> (\<exists>m'\<in>semantics p m. B m'))"
-
-lemma hoare_skip[simp]: "hoare A [] A"
-  unfolding hoare_def by auto
-
-lemma hoare_cons: 
-  assumes "hoare A [c] B"
-  assumes "hoare B p C"
-  shows "hoare A (c#p) C"
-  using assms unfolding hoare_def apply auto by metis
-
-lemma hoareI:
-  assumes "\<And>m. A m \<Longrightarrow> Bex (semantics p m) B"
-  shows "hoare A p B"
-  unfolding hoare_def using assms by simp
-
-lemma valid_Add:
-  assumes "B \<equiv> postcondition_trivial (Add x y) A"
-  assumes "p \<equiv> [Add x y]"
-  assumes distinct: "x \<noteq> y"
-  shows "hoare A p B"
-  apply (rule hoareI)
-  unfolding assms(1-2) using distinct by simp
-
-
-lemma valid_Set:
-  assumes "B \<equiv> postcondition_trivial (Set x i) A"
-  assumes "p \<equiv> [Set x i]"
-  shows "hoare A p B"
-  apply (rule hoareI)
-  unfolding assms
-  apply simp
-  by (metis fun_upd_triv)
-
-lemma valid_Guess_trivial:
-  assumes "B \<equiv> postcondition_trivial (Guess x) A"
-  assumes "p == [Guess x]"
-  shows "hoare A p B"
-  apply (rule hoareI)
-  unfolding assms
-  apply simp
-  by (metis fun_upd_triv)
-
-lemma valid_Guess_pick:
-  assumes "B \<equiv> postcondition_pick (Guess x) i A"
-  assumes "p == [Guess x]"
-  shows "hoare A p B"
-  apply (rule hoareI)
-  unfolding assms
-  apply (rule bexI[of _ "_(x := i)"])
-  apply auto
-  by (metis fun_upd_triv)
-
-lemmas valid = valid_Set valid_Guess_pick valid_Guess_trivial valid_Add
-
 ML \<open>
-fun use_facts_tac ctxt thms = 
-  EVERY' (map (fn thm => forward_tac ctxt [thm COMP @{thm pc_impD}]) (rev (tl thms)))
-  THEN' (dresolve_tac ctxt [hd thms COMP @{thm pc_impD}])
-\<close>
 
-lemma list_rev_induct2 [consumes 1, case_names Nil snoc]:
-  "length xs = length ys \<Longrightarrow> P [] [] \<Longrightarrow>
-   (\<And>x xs y ys. length xs = length ys \<Longrightarrow> P xs ys \<Longrightarrow> P (xs@[x]) (ys@[y]))
-   \<Longrightarrow> P xs ys"
-  apply (rule list_induct2[where xs="rev xs" and ys="rev ys" and P="\<lambda>xs ys. P (rev xs) (rev ys)", simplified])
-  by auto
-
-lemma hoare_conseq:
-  assumes "pc_imp A A'"
-  assumes "pc_imp B' B"
-  assumes "hoare A' p B'"
-  shows "hoare A p B"
-  using assms unfolding hoare_def pc_imp_def by blast
-
-lemma hoare_conseq':
-  assumes "hoare A' p' B'"
-  assumes "pc_imp A A'"
-  assumes "pc_imp B' B"
-  assumes "p = p'"
-  shows "hoare A p B"
-  using assms unfolding hoare_def pc_imp_def by blast
-
-ML \<open>
 fun hoare_thm ctxt (hoare:hoare) : cterm = let
-  (* val hoare = get_hoare ctxt hoare |> the *)
+  val logic = hoare |> #program |> get_program ctxt |> the |> #logic |> get_logic' ctxt |> the
   val pre = #precondition hoare |> get_invariant ctxt |> the |> #const
   val post = #postcondition hoare |> get_invariant ctxt |> the |> #const
   val prog = #program_fragment_const hoare
-  val prop = \<^const>\<open>hoare\<close> $ pre $ prog $ post |> HOLogic.mk_Trueprop
+  val prop = #hoare_thm logic ctxt pre prog post
   in Thm.cterm_of ctxt prop end
 \<close>
 
 ML \<open>
-fun update_hoare_valid new_valid ({binding, range, program_fragment, program_fragment_const, precondition,
-  postcondition, valid=_}:hoare) : hoare =
- {binding=binding, range=range, program_fragment=program_fragment,
-  program_fragment_const=program_fragment_const, precondition=precondition,
-  postcondition=postcondition,
-  valid=new_valid}
+fun update_hoare_valid new_valid ({binding, range, program_fragment_const, precondition,
+  postcondition, program, valid=_}:hoare) : hoare =
+   {binding=binding, range=range, 
+    program_fragment_const=program_fragment_const, precondition=precondition,
+    postcondition=postcondition,
+    program=program,
+    valid=new_valid}
 \<close>
 
 
 ML \<open>
-fun add_hoare2 binding program range (precondition:invariant) (postcondition:invariant) state : hoare * Proof.state = let
+fun add_hoare2 binding (program:program) range (precondition:invariant) (postcondition:invariant) state : hoare * Proof.state = let
   val (info,state) = Proof.map_context_result (add_hoare1 binding program range precondition postcondition) state
   fun after_qed (_,[[valid]]) = Proof.map_context (add_hoare0 (update_hoare_valid valid info))
   val valid_prop = hoare_thm (Proof.context_of state) info |> Thm.term_of
@@ -398,116 +265,20 @@ fun add_hoare2 binding program range (precondition:invariant) (postcondition:inv
   in (info,state) end
 \<close>
 
-lemma semantics_seq: "semantics (p@q) m = 
-  (\<Union>m'\<in>semantics p m. semantics q m')"
-  sorry
 
-lemma hoare_seq:
-  assumes "hoare A p B"
-  assumes "hoare B q C"
-  shows "hoare A (p@q) C"
-proof (unfold hoare_def, auto)
-  fix m
-  assume "A m"
-  with assms(1) obtain m' where "B m'" and m': "m' \<in> semantics p m"
-    apply atomize_elim unfolding hoare_def by auto
-  with assms(2) obtain m'' where "C m''" and m'': "m'' \<in> semantics q m'"
-    apply atomize_elim unfolding hoare_def by auto
-  from m' m'' have "m'' \<in> semantics (p@q) m"
-    unfolding semantics_seq by auto
-  with \<open>C m''\<close> show "\<exists>m''\<in>semantics (p@q) m. C m''"
-    by auto
-qed
-
-lemma hoare_seq':
-  assumes "hoare A p B"
-  assumes "hoare B q C"
-  assumes "pq = p @ q"
-  shows "hoare A pq C"
-  unfolding assms(3) using assms(1-2) by (rule hoare_seq) 
-
-lemma True
-proof 
-
-  define prog where "prog = [Set STR ''x'' 5, Guess STR ''y'', Add STR ''x'' STR ''y'']"
-
-  do_prf \<open>fn state => let
-    val (start_invariant,state) = Proof.map_context_result (add_invariant \<^binding>\<open>start\<close> \<^cterm>\<open>(\<lambda>m::mem. True)\<close>) state
-    val (hoare,state) = add_hoare2 \<^binding>\<open>start\<close> test_prog (0,0) start_invariant start_invariant state
-    val _ = \<^print> hoare
-    in state end\<close>
-
-    unfolding start_prog_def by simp
-
-  (* Step 1: Set x 5 *)
-
-  do_prf \<open>fn state => let
-    val (post,state) = Proof.map_context_result (add_invariant \<^binding>\<open>step1\<close> \<^cterm>\<open>(postcondition_trivial (Set STR ''x'' 5) start_inv)\<close>) state
-    val start = get_invariant (Proof.context_of state) "start" |> the
-    val (hoare,state) = add_hoare2 \<^binding>\<open>step1\<close> test_prog (0,1) start post state
-    in state end\<close>
-    using step1_inv_def step1_prog_def by (rule valid)
-
-  have step1_x5: "pc_imp step1_inv (\<lambda>m. m STR ''x'' = 5)"
-    using step1_inv_def by (rule newvalue)
-
-  (* Step 2: Guess y *)
-
-  do_prf \<open>fn state => let
-    val (post,state) = Proof.map_context_result (add_invariant \<^binding>\<open>step2\<close>
-         \<^cterm>\<open>postcondition_pick (Guess STR ''y'') (-5) step1_inv\<close>) state
-    val pre = get_invariant (Proof.context_of state) "step1" |> the
-    val (hoare,state) = add_hoare2 \<^binding>\<open>step2\<close> test_prog (1,2) pre post state
-    in state end\<close>
-    using step2_inv_def step2_prog_def by (rule valid)
-
-  have step2_x5: "pc_imp step2_inv (\<lambda>m. m STR ''x'' = 5)"
-    using step2_inv_def apply (rule unchanged)
-     apply (rule independent_ofI, simp)
-    apply (tactic \<open>use_facts_tac \<^context> @{thms step1_x5} 1\<close>)
-    by simp
-
-  have step2_y5: "pc_imp step2_inv (\<lambda>m. m STR ''y'' = -5)"
-    using step2_inv_def by (rule newvalue)
-
-  have start_step2: "hoare start_inv (step1_prog @ step2_prog) step2_inv"
-    using step1_valid step2_valid by (rule hoare_seq)    
-
-  (* Step 3: Add x y *)
-
-  do_prf \<open>fn state => let
-    val (post,state) = Proof.map_context_result (add_invariant \<^binding>\<open>step3\<close>
-       \<^cterm>\<open>(postcondition_trivial (Add STR ''x'' STR ''y'') step2_inv)\<close>) state
-    val pre = get_invariant (Proof.context_of state) "step2" |> the
-    val (hoare,state) = add_hoare2 \<^binding>\<open>step3\<close> test_prog (2,3) pre post state
-    in state end\<close>
-    using step3_inv_def step3_prog_def by (rule valid, simp)
-
-  have step3_y5: "pc_imp step3_inv (\<lambda>m. m STR ''y'' = -5)"
-    using step3_inv_def apply (rule unchanged)
-      apply (rule independent_ofI, simp)
-     apply simp
-    apply (tactic \<open>use_facts_tac \<^context> @{thms step2_y5} 1\<close>)
-    by simp
-
-  have step3_x0: "pc_imp step3_inv (\<lambda>m. m STR ''x'' = 0)"
-    using step3_inv_def apply (rule wp)
-     apply simp
-    apply (tactic \<open>use_facts_tac \<^context> @{thms step2_x5 step2_y5} 1\<close>)
-    by simp
-
-  have start_step3: "hoare start_inv prog step3_inv"
-    using start_step2 step3_valid
-    apply (rule hoare_seq')
-    by (simp add: prog_def step1_prog_def step2_prog_def step3_prog_def)
-
-  then have "hoare (\<lambda>_. True) prog (\<lambda>m. m STR ''x'' = 0)"
-    apply (rule hoare_conseq')
-    unfolding start_inv_def apply (simp add: pc_imp_def)
-     apply (rule step3_x0)
-    by simp
-
-qed
+ML \<open>
+fun add_hoare3 binding (program:string option) range (precondition:string) (postcondition:term) state = let
+    val ctxt = Proof.context_of state
+    val program = case program of 
+      SOME program => program
+    | NONE => get_current_program ctxt |> the
+    val program = get_program ctxt program |> the
+    val precondition = case get_invariant (Proof.context_of state) precondition of
+      SOME inv => inv | NONE => error ("Undefined precondition " ^ precondition)
+    val (postcondition,state) = Proof.map_context_result (add_invariant binding postcondition) state
+    val (_,state) = add_hoare2 binding program range precondition postcondition state
+in state end
+\<close>
 
 
 end
