Demo_Hoare.thy
@@ -1,0 +1,272 @@
+theory Demo_Hoare
+  imports Forward_Hoare
+begin
+
+
+ML \<open>
+datatype instruction = Add of var*var | Set of var*int | Guess of var
+  fun instruction_to_term (Set (x, i)) = \<^const>\<open>Set\<close> $ HOLogic.mk_literal x $ HOLogic.mk_number HOLogic.intT i
+    | instruction_to_term (Guess x) = \<^const>\<open>Guess\<close> $ HOLogic.mk_literal x
+    | instruction_to_term (Add (x,y)) = \<^const>\<open>Add\<close> $ HOLogic.mk_literal x $ HOLogic.mk_literal y
+  fun program_to_term p = map instruction_to_term p |> HOLogic.mk_list \<^typ>\<open>instruction\<close>
+\<close>
+
+fun semantics1 :: "instruction \<Rightarrow> mem \<Rightarrow> mem set" where
+  "semantics1 (Set x i) m = {m(x:=i)}"
+| "semantics1 (Add x y) m = {m(x:=m x + m y)}"
+| "semantics1 (Guess x) m = {m(x:=i)| i. True}"
+
+fun semantics :: "program \<Rightarrow> mem \<Rightarrow> mem set" where
+  "semantics [] m = {m}"
+| "semantics (c#p) m = (\<Union>m'\<in>semantics1 c m. semantics p m')"
+
+type_synonym invariant = "mem \<Rightarrow> bool"
+
+definition hoare :: "invariant \<Rightarrow> program \<Rightarrow> invariant \<Rightarrow> bool" where
+  "hoare A p B \<longleftrightarrow> (\<forall>m. A m \<longrightarrow> (\<exists>m'\<in>semantics p m. B m'))"
+
+
+ML \<open>
+structure Demo_Hoare_Logic = Hoare_Logic(
+  type program = instruction list
+  type range = int * int
+
+  val binding = \<^binding>\<open>demo_logic\<close>
+
+  fun read_program ctxt str = error "read_program"
+  fun read_range ctxt str = error "read_range"
+
+  fun hoare_thm ctxt pre prog post = \<^const>\<open>hoare\<close> $ pre $ prog $ post |> HOLogic.mk_Trueprop
+
+  fun valid_range (program:program) ((start,endd):range) =
+    start <= endd andalso start >= 0 andalso endd <= length program
+
+  fun extract_range (program:program) ((start,endd):range) : term =
+    program |> drop start |> take (endd-start) |> program_to_term
+)
+\<close>
+
+
+fun postcondition_trivial :: "instruction \<Rightarrow> invariant \<Rightarrow> invariant" where
+  "postcondition_trivial (Set x i) I = (\<lambda>m. m x = i \<and> (\<exists>j. I (m(x:=j))))"
+| "postcondition_trivial (Guess x) I = (\<lambda>m. \<exists>j. I (m(x:=j)))"
+| "postcondition_trivial (Add x y) I = (\<lambda>m. I (m(x:=m x - m y)))"
+
+fun postcondition_pick :: "instruction \<Rightarrow> int \<Rightarrow> invariant \<Rightarrow> invariant" where
+  "postcondition_pick (Guess x) i I = (\<lambda>m. m x = i \<and> (\<exists>j. I (m(x:=j))))"
+| "postcondition_pick _ _ _ = undefined"
+
+lemma semantics_seq: "semantics (p@q) m = 
+  (\<Union>m'\<in>semantics p m. semantics q m')"
+  by (induction p arbitrary: m, auto)
+
+lemma hoare_seq:
+  assumes "hoare A p B"
+  assumes "hoare B q C"
+  shows "hoare A (p@q) C"
+proof (unfold hoare_def, auto)
+  fix m
+  assume "A m"
+  with assms(1) obtain m' where "B m'" and m': "m' \<in> semantics p m"
+    apply atomize_elim unfolding hoare_def by auto
+  with assms(2) obtain m'' where "C m''" and m'': "m'' \<in> semantics q m'"
+    apply atomize_elim unfolding hoare_def by auto
+  from m' m'' have "m'' \<in> semantics (p@q) m"
+    unfolding semantics_seq by auto
+  with \<open>C m''\<close> show "\<exists>m''\<in>semantics (p@q) m. C m''"
+    by auto
+qed
+
+lemma hoare_seq':
+  assumes "hoare A p B"
+  assumes "hoare B q C"
+  assumes "pq = p @ q"
+  shows "hoare A pq C"
+  unfolding assms(3) using assms(1-2) by (rule hoare_seq) 
+
+
+definition "pc_imp pc1 pc2 \<longleftrightarrow> (\<forall>m. pc1 m \<longrightarrow> pc2 m)"
+
+lemma pc_impI[intro]: "(\<And>m. pc1 m \<Longrightarrow> pc2 m) \<Longrightarrow> pc_imp pc1 pc2"
+  unfolding pc_imp_def by auto
+
+lemma pc_impD[dest]: "pc_imp pc1 pc2 \<Longrightarrow> pc1 m \<Longrightarrow> pc2 m"
+  unfolding pc_imp_def by auto
+
+ML \<open>
+fun use_facts_tac ctxt thms = 
+  EVERY' (map (fn thm => forward_tac ctxt [thm COMP @{thm pc_impD}]) (rev (tl thms)))
+  THEN' (dresolve_tac ctxt [hd thms COMP @{thm pc_impD}])
+\<close>
+
+lemma hoare_conseq:
+  assumes "pc_imp A A'"
+  assumes "pc_imp B' B"
+  assumes "hoare A' p B'"
+  shows "hoare A p B"
+  using assms unfolding hoare_def pc_imp_def by blast
+
+lemma hoare_conseq':
+  assumes "hoare A' p' B'"
+  assumes "pc_imp A A'"
+  assumes "pc_imp B' B"
+  assumes "p = p'"
+  shows "hoare A p B"
+  using assms unfolding hoare_def pc_imp_def by blast
+
+
+lemma hoare_skip[simp]: "hoare A [] A"
+  unfolding hoare_def by auto
+
+lemma hoare_cons: 
+  assumes "hoare A [c] B"
+  assumes "hoare B p C"
+  shows "hoare A (c#p) C"
+  using assms unfolding hoare_def apply auto by metis
+
+lemma hoareI:
+  assumes "\<And>m. A m \<Longrightarrow> Bex (semantics p m) B"
+  shows "hoare A p B"
+  unfolding hoare_def using assms by simp
+
+lemma valid_Add:
+  assumes "B \<equiv> postcondition_trivial (Add x y) A"
+  assumes "p \<equiv> [Add x y]"
+  assumes distinct: "x \<noteq> y"
+  shows "hoare A p B"
+  apply (rule hoareI)
+  unfolding assms(1-2) using distinct by simp
+
+
+lemma valid_Set:
+  assumes "B \<equiv> postcondition_trivial (Set x i) A"
+  assumes "p \<equiv> [Set x i]"
+  shows "hoare A p B"
+  apply (rule hoareI)
+  unfolding assms
+  apply simp
+  by (metis fun_upd_triv)
+
+lemma valid_Guess_trivial:
+  assumes "B \<equiv> postcondition_trivial (Guess x) A"
+  assumes "p == [Guess x]"
+  shows "hoare A p B"
+  apply (rule hoareI)
+  unfolding assms
+  apply simp
+  by (metis fun_upd_triv)
+
+lemma valid_Guess_pick:
+  assumes "B \<equiv> postcondition_pick (Guess x) i A"
+  assumes "p == [Guess x]"
+  shows "hoare A p B"
+  apply (rule hoareI)
+  unfolding assms
+  apply (rule bexI[of _ "_(x := i)"])
+  apply auto
+  by (metis fun_upd_triv)
+
+lemmas valid = valid_Set valid_Guess_pick valid_Guess_trivial valid_Add
+
+
+
+definition "independent_of (B::invariant) (x::var) = (\<forall>m1 m2. (\<forall>y\<noteq>x. m1 y = m2 y) \<longrightarrow> B m1 = B m2)"
+lemma independent_ofI: 
+  assumes "\<And>m1 m2. (\<And>y. y\<noteq>x \<Longrightarrow> m1 y = m2 y) \<Longrightarrow> B m1 = B m2"
+  shows "independent_of B x"
+  unfolding independent_of_def using assms by metis
+
+lemma newvalue_Set:
+  assumes "invariant \<equiv> postcondition_trivial (Set x i) A"
+  shows "pc_imp invariant (\<lambda>m. m x = i)"
+  unfolding assms
+  by (rule pc_impI; simp)
+
+lemma newvalue_Guess: 
+  assumes "invariant \<equiv> postcondition_pick (Guess x) i A"
+  shows "pc_imp invariant (\<lambda>m. m x = i)"
+  unfolding assms
+  by (rule pc_impI; simp)
+
+lemmas newvalue = newvalue_Set newvalue_Guess
+
+lemma unchanged_Guess_trivial: 
+  assumes "invariant \<equiv> postcondition_trivial (Guess x) A"
+  assumes indep: "independent_of B x"
+  assumes imp: "\<And>m. A m \<Longrightarrow> B m"
+  shows "pc_imp invariant B"
+  unfolding assms(1)
+  apply (rule pc_impI; simp)
+  using indep imp unfolding independent_of_def apply auto
+  by (metis fun_upd_def)+
+
+lemma unchanged_Guess_pick: 
+  assumes "invariant \<equiv> postcondition_pick (Guess x) i A"
+  assumes indep: "independent_of B x"
+  assumes imp: "\<And>m. A m \<Longrightarrow> B m"
+  shows "pc_imp invariant B"
+  unfolding assms(1)
+  apply (rule pc_impI; simp)
+  using indep imp unfolding independent_of_def apply auto
+  by (metis fun_upd_def)+
+
+lemma unchanged_Add: 
+  assumes "invariant \<equiv> postcondition_trivial (Add x y) A"
+  assumes indep: "independent_of B x"
+  assumes xy: "x \<noteq> y"
+  assumes imp: "\<And>m. A m \<Longrightarrow> B m"
+  shows "pc_imp invariant B"
+  unfolding assms
+  apply (rule pc_impI)
+  using indep imp xy unfolding independent_of_def apply auto
+  by (metis fun_upd_def)
+
+lemma unchanged_Set: 
+  assumes "invariant \<equiv> postcondition_trivial (Set x i) A"
+  assumes indep: "independent_of B x"
+  assumes imp: "\<And>m. A m \<Longrightarrow> B m"
+  shows "pc_imp invariant B"
+  unfolding assms(1)
+  apply (rule pc_impI)
+  using indep imp unfolding independent_of_def apply auto
+  by (metis fun_upd_def)
+
+lemmas unchanged = unchanged_Guess_pick unchanged_Guess_trivial unchanged_Add unchanged_Set
+
+lemma wp_Add: 
+  assumes "invariant \<equiv> postcondition_trivial (Add x y) A"
+  assumes distinct: "x \<noteq> y"
+  assumes imp: "\<And>m. A m \<Longrightarrow> B (m(x:=m x + m y))"
+  shows "pc_imp invariant B"
+  unfolding assms(1)
+  apply (rule pc_impI)
+  using distinct apply simp apply (drule imp)
+  by auto
+
+lemma wp_Set:
+  assumes "invariant \<equiv> postcondition_trivial (Set x i) A"
+  assumes imp: "\<And>m. A m \<Longrightarrow> B (m(x:=i))"
+  shows "pc_imp invariant B"
+  unfolding assms(1)
+  apply (rule pc_impI)
+  apply simp
+  using imp
+  apply auto
+  apply (drule imp)
+  by auto
+
+lemmas wp = wp_Add wp_Set
+
+
+
+ML \<open>
+
+(* Contract: valid_range = true *)
+(* fun merge_ranges (_:program) ((s1,e1):Demo_Hoare_Logic.range) ((s2,e2):range) : range option =
+  if e1=s2 then SOME (s1,e2) else NONE *)
+\<close>
+
+
+
+
+end
