Test.thy
@@ -1,0 +1,78 @@
+theory Test
+  imports Demo_Hoare
+begin
+
+
+lemma True
+proof 
+
+  do \<open>fn ctxt => let
+    val prog = Demo_Hoare_Logic.ex_program [Set ("x", 5), Guess "y", Add ("x", "y")]
+    val ctxt = add_program0 {binding=\<^binding>\<open>prog\<close>, logic="demo_logic", code=prog} ctxt
+    in ctxt end\<close>
+
+  define prog where "prog = [Set STR ''x'' 5, Guess STR ''y'', Add STR ''x'' STR ''y'']"
+
+  do \<open>snd o add_invariant \<^binding>\<open>start\<close> \<^term>\<open>(\<lambda>m::mem. True)\<close>\<close>
+
+  (* Step 1: Set x 5 *)
+
+  do_prf \<open>add_hoare3 \<^binding>\<open>step1\<close> NONE (Demo_Hoare_Logic.ex_range (0,1)) "start"
+     \<^term>\<open>(postcondition_trivial (Set STR ''x'' 5) start_inv)\<close>\<close>
+    using step1_inv_def step1_prog_def by (rule valid)
+
+  have step1_x5: "pc_imp step1_inv (\<lambda>m. m STR ''x'' = 5)"
+    using step1_inv_def by (rule newvalue)
+
+  (* Step 2: Guess y *)
+
+  do_prf \<open>add_hoare3 \<^binding>\<open>step2\<close> NONE (Demo_Hoare_Logic.ex_range (1,2)) "step1"
+    \<^term>\<open>postcondition_pick (Guess STR ''y'') (-5) step1_inv\<close>\<close>
+    using step2_inv_def step2_prog_def by (rule valid)
+
+  have step2_x5: "pc_imp step2_inv (\<lambda>m. m STR ''x'' = 5)"
+    using step2_inv_def apply (rule unchanged)
+     apply (rule independent_ofI, simp)
+    apply (tactic \<open>use_facts_tac \<^context> @{thms step1_x5} 1\<close>)
+    by simp
+
+  have step2_y5: "pc_imp step2_inv (\<lambda>m. m STR ''y'' = -5)"
+    using step2_inv_def by (rule newvalue)
+
+  have start_step2: "hoare start_inv (step1_prog @ step2_prog) step2_inv"
+    using step1_valid step2_valid by (rule hoare_seq)    
+
+  (* Step 3: Add x y *)
+
+  do_prf \<open>add_hoare3 \<^binding>\<open>step3\<close> NONE (Demo_Hoare_Logic.ex_range (2,3)) "step2"
+    \<^term>\<open>(postcondition_trivial (Add STR ''x'' STR ''y'') step2_inv)\<close>\<close>
+    using step3_inv_def step3_prog_def by (rule valid, simp)
+
+  have step3_y5: "pc_imp step3_inv (\<lambda>m. m STR ''y'' = -5)"
+    using step3_inv_def apply (rule unchanged)
+      apply (rule independent_ofI, simp)
+     apply simp
+    apply (tactic \<open>use_facts_tac \<^context> @{thms step2_y5} 1\<close>)
+    by simp
+
+  have step3_x0: "pc_imp step3_inv (\<lambda>m. m STR ''x'' = 0)"
+    using step3_inv_def apply (rule wp)
+     apply simp
+    apply (tactic \<open>use_facts_tac \<^context> @{thms step2_x5 step2_y5} 1\<close>)
+    by simp
+
+  have start_step3: "hoare start_inv prog step3_inv"
+    using start_step2 step3_valid
+    apply (rule hoare_seq')
+    by (simp add: prog_def step1_prog_def step2_prog_def step3_prog_def)
+
+  then have "hoare (\<lambda>_. True) prog (\<lambda>m. m STR ''x'' = 0)"
+    apply (rule hoare_conseq')
+    unfolding start_inv_def apply (simp add: pc_imp_def)
+     apply (rule step3_x0)
+    by simp
+
+qed
+
+
+end
